src/Dflatmajortocmajor.v
@@ -65,11 +65,10 @@ Definition transf_fundef (alloc : ident) (fd : Dmajor.fundef) : res Cmajor.funde
   OK (AST.transf_fundef (transf_function alloc) fd).
 
 
-Definition new_globs (bump : ident) (alloc : ident) : list (ident * globdef Cmajor.fundef unit) :=
-    nil.
+(*Definition new_globs (bump : ident) (alloc : ident) : list (ident * globdef Cmajor.fundef unit) := nil.*)
                                                            
 
-Fixpoint largest_id (x : ident) (l : list ident) : ident :=
+(*Fixpoint largest_id (x : ident) (l : list ident) : ident :=
   match l with
   | nil => x
   | f :: r =>
@@ -77,17 +76,41 @@ Fixpoint largest_id (x : ident) (l : list ident) : ident :=
   end.
 
 Definition largest_id_prog (prog : Dmajor.program) : ident :=
-  largest_id (1%positive) (map fst (prog_defs prog)).
+  largest_id (1%positive) (map fst (prog_defs prog)).*)
 
 Axiom register_ident_as_malloc : positive -> positive.
 Axiom register_ident_as_malloc_is_id : forall p, register_ident_as_malloc p = p.
 Extract Inlined Constant register_ident_as_malloc => "Camlcoq.register_ident_as_malloc".
 
-Definition transf_prog (prog : Dmajor.program) : res Cmajor.program :=
-  let malloc_id := register_ident_as_malloc (Pos.succ (largest_id_prog prog)) in
-  let bump := Pos.succ malloc_id in
-  transform_partial_augment_program (transf_fundef malloc_id) (fun x => OK x)
-                                    (new_globs bump malloc_id) (prog_main prog) prog.
+Definition transf_prog (prog : Dmajor.program) (malloc_id : ident) : res Cmajor.program :=
+  transform_partial_program (transf_fundef malloc_id) prog.
+
+
+Lemma plus_left_e :
+  forall {F V} {state : Type} (tge : Genv.t F V) (step : Genv.t F V -> state -> trace -> state -> Prop) (st st' : state) P,
+    step tge st E0 st' ->
+    (exists ste,
+        star step tge st' E0 ste /\ P ste) ->
+    (exists ste,
+        plus step tge st E0 ste /\ P ste).
+Proof.
+  intros. break_exists. break_and.
+  eexists; split; try eassumption.
+  eapply plus_left; eauto.
+Qed.
+
+Lemma star_left_e :
+  forall {F V} {state : Type} (tge : Genv.t F V) (step : Genv.t F V -> state -> trace -> state -> Prop) (st st' : state) P,
+    step tge st E0 st' ->
+    (exists ste,
+        star step tge st' E0 ste /\ P ste) ->
+    (exists ste,
+        star step tge st E0 ste /\ P ste).
+Proof.
+  intros. break_exists. break_and.
+  eexists; split; try eassumption.
+  eapply star_left; eauto.
+Qed.
 
 
 Section PRESERVATION.
@@ -96,32 +119,13 @@ Variable prog: Dmajor.program.
 Variable tprog: Cmajor.program.
 Let ge := Genv.globalenv prog.
 Let tge := Genv.globalenv tprog.
-Hypothesis TRANSF : transf_prog prog = OK tprog.
-Hypothesis NOREP : list_norepet (prog_defs_names prog).
-Definition malloc_id := register_ident_as_malloc (Pos.succ (largest_id_prog prog)).
-Hypothesis NEW_GLOBS_NOT_PUBLIC :
-  forall id,
-    In id (map fst (new_globs (Pos.succ malloc_id) malloc_id)) ->
-   ~ In id (Genv.genv_public tge).
-
-
-
-
-Lemma match_prog :
-  match_program
-             (fun (fd : fundef) (tfd : Cmajor.fundef) =>
-              transf_fundef malloc_id fd = OK tfd)
-             (fun info tinfo : unit => OK info = OK tinfo)
-             (new_globs (Pos.succ malloc_id) malloc_id) (prog_main prog) prog tprog.
-Proof.
-  intros.
-  unfold transf_prog in TRANSF.
-  app transform_partial_augment_program_match transform_partial_augment_program.
-Qed.
-
-(* extensionally equal environments *)
-Definition env_lessdef (e1 e2: env) : Prop :=
-  forall id v1, e1!id = Some v1 -> exists v2, e2!id = Some v2 /\ Val.lessdef v1 v2.
+Hypothesis malloc_id : ident.
+Hypothesis TRANSF : transf_prog prog malloc_id = OK tprog.
+Hypothesis malloc_block : block.
+Hypothesis malloc_id_malloc :
+  Genv.find_symbol ge malloc_id = Some malloc_block.
+Hypothesis malloc_block_malloc :
+  Genv.find_funct_ptr ge malloc_block = Some (External (EF_malloc)).
 
 Inductive match_cont: Dflatmajor.cont -> Cmajor.cont -> Prop :=
   | match_cont_stop:
@@ -134,37 +138,37 @@ Inductive match_cont: Dflatmajor.cont -> Cmajor.cont -> Prop :=
       transf_stmt malloc_id s = s' ->
       match_cont k k' ->
       match_cont (Dflatmajor.Kseq s k) (Cmajor.Kseq s' k')
-  | match_cont_call: forall id f sp e k f' e' k',
+  | match_cont_call: forall id f sp e k f' k',
       transf_function malloc_id f = f' ->
       match_cont k k' ->
-      env_lessdef e e' ->
-      match_cont (Dflatmajor.Kcall id f sp e k) (Cmajor.Kcall id f' sp e' k').
+      (*env_lessdef e e' ->*)
+      match_cont (Dflatmajor.Kcall id f sp e k) (Cmajor.Kcall id f' sp e k').
 
 Inductive match_states : Dflatmajor.state -> Cmajor.state -> Prop :=
-  | match_state: forall f f' s k s' k' sp e m e' m' z
+  | match_state: forall f f' s k s' k' sp e m z
         (TF: transf_function malloc_id f = f')
         (TS: transf_stmt malloc_id s = s')
-        (MC: match_cont k k')
-        (LD: env_lessdef e e')
-        (ME: Mem.extends m m'),
+        (MC: match_cont k k'),
+        (*(LD: env_lessdef e e')*)
+        (*(ME: Mem.extends m m'),*)
       match_states
         (Dflatmajor.State f s k sp e m z)
-        (Cmajor.State f' s' k' sp e' m')
-  | match_callstate: forall f f' args args' k k' m m' z
+        (Cmajor.State f' s' k' sp e m)
+  | match_callstate: forall f f' args k k' m z
         (TF: transf_fundef malloc_id (Internal f) = OK f')
-        (MC: match_cont k k')
-        (LD: Val.lessdef_list args args')
-        (ME: Mem.extends m m'),
+        (MC: match_cont k k'),
+        (*(LD: Val.lessdef_list args args')*)
+        (*(ME: Mem.extends m m'),*)
       match_states
         (Dflatmajor.Callstate f args k m z)
-        (Cmajor.Callstate f' args' k' m')
-  | match_returnstate: forall v v' k k' m m' z
-        (MC: match_cont k k')
-        (LD: Val.lessdef v v')
-        (ME: Mem.extends m m'),
+        (Cmajor.Callstate f' args k' m)
+  | match_returnstate: forall v k k' m z
+        (MC: match_cont k k'),
+        (*(LD: Val.lessdef v v')
+        (ME: Mem.extends m m'),*)
       match_states
         (Dflatmajor.Returnstate v k m z)
-        (Cmajor.Returnstate v' k' m').
+        (Cmajor.Returnstate v k' m).
 
 Remark call_cont_commut:
   forall k k', match_cont k k' -> match_cont (Dflatmajor.call_cont k) (Cmajor.call_cont k').
@@ -196,7 +200,7 @@ Ltac break_or :=
   match goal with
   | [ H : _ \/ _ |- _ ] => destruct H
   end.
-
+(*
 Lemma largest_id_base :
   forall l base,
     (base <= (largest_id base l))%positive.
@@ -209,13 +213,13 @@ Proof.
   eapply IHl.
   eapply IHl.
 Qed.
-
+*)
 Ltac use H :=
   let HH := fresh "H" in
   let H2 := fresh "H" in
   remember H as H2 eqn:HH;
   clear HH.
-
+(*
 Lemma not_Plt_Ple :
   forall a b,
     ~ Plt a b ->
@@ -274,117 +278,60 @@ Lemma new_globs_id :
     In id (map fst (new_globs (Pos.succ bound) bound)) ->
     (bound <= id)%positive.
 Proof.
-Admitted.
 
+*)
 Lemma find_symbol_transf :
-  forall id x,
-    Genv.find_symbol ge id = Some x ->
-    Genv.find_symbol tge id = Some x.
-Proof.
-Admitted.
-
-
-Lemma eval_const_transf_lessdef :
-  forall sp c v,
-    Dflatmajor.eval_constant ge sp c = Some v ->
-    exists v',
-      Cmajor.eval_constant tge sp (transf_const c) = Some v' /\ Val.lessdef v v'.
+  forall id,
+    Genv.find_symbol tge id = Genv.find_symbol ge id.
 Proof.
   intros.
-  destruct c; simpl in *; eauto.
-  break_match_hyp. app find_symbol_transf Genv.find_symbol.
-  collapse_match. eauto.
-  break_match; eauto.
-  inv H. eauto.
+  unfold ge, tge in *.
+  unfold transf_prog in *.
+  erewrite Genv.find_symbol_transf_partial; eauto.
 Qed.
 
 Lemma eval_expr_transf :
   forall sp a e m v,
     Dflatmajor.eval_expr ge e m sp a v ->
-    forall e' m',
-      env_lessdef e e' ->
-      Mem.extends m m' ->
-      exists v',
-        Cmajor.eval_expr tge e' m' sp (transf_expr a) v' /\ Val.lessdef v v'.
+    Cmajor.eval_expr tge e m sp (transf_expr a) v.
 Proof.
-  induction a; intros.
-  * inv H.
-    unfold env_lessdef in *.
-    apply H0 in H3. break_exists. break_and.
-    eexists.
-    split. econstructor.
-    eassumption. assumption.
-  * inversion H.
-    app eval_const_transf_lessdef eval_constant.
-    exists x. split; eauto. simpl.
-    econstructor; eauto.
-    
-  * inv H.
-    eapply IHa1 in H4; eauto.
-    eapply IHa2 in H6; eauto.
-    clear IHa1 IHa2.
-    repeat break_exists; repeat break_and.
-    exists (Val.add x0 x). split.
-    simpl. econstructor; eauto.
-    eapply Val.add_lessdef; eauto.
-  * inv H. eapply IHa in H4; eauto.
-    break_exists. break_and.
-    clear IHa.
-    simpl.
-    eapply Mem.loadv_extends in H6; eauto.
-    break_exists; break_and. 
-    exists x0. split; eauto.
-    econstructor; eauto.
+  induction a; intros; simpl; invp eval_expr;
+    try solve [econstructor; eauto].
+  subst. simpl.
+  econstructor; eauto.
+  destruct c; simpl in H1; inv H1; simpl; auto.
+  repeat break_match_hyp; try congruence;
+    erewrite find_symbol_transf; repeat collapse_match; eauto.
 Qed.
 
 Lemma eval_exprlist_transf :
   forall a sp e m v,
     Dflatmajor.eval_exprlist ge e m sp a v ->
-    forall e' m',
-      env_lessdef e e' ->
-      Mem.extends m m' ->
-      exists v',
-        Cmajor.eval_exprlist tge e' m' sp (map transf_expr a) v' /\ Val.lessdef_list v v'.
+    Cmajor.eval_exprlist tge e m sp (map transf_expr a) v.    
 Proof.
   induction a; intros.
-  inversion H. subst v. eexists; split; econstructor; eauto.
+  inversion H. subst v.
+  econstructor; eauto.
   inversion H.
   remember tprog. subst.
-  eapply IHa in H6; eauto.
+  eapply IHa in H4; eauto.
   repeat break_exists; repeat break_and.
-  eapply eval_expr_transf in H4; eauto.
+  eapply eval_expr_transf in H2; eauto.
   repeat break_exists; repeat break_and.
-  eexists; split; try econstructor; eauto.
+  econstructor; eauto.
 Qed.  
-
-Lemma env_lessdef_set :
-  forall id v v' e e',
-    Val.lessdef v v' ->
-    env_lessdef e e' ->
-    env_lessdef (PTree.set id v e) (PTree.set id v' e').
-Proof.
-  intros.
-  unfold env_lessdef in *.
-  intros.
-  destruct (peq id id0); subst.
-  rewrite PTree.gss in *. eexists; split; eauto. congruence.
-  rewrite PTree.gso in * by congruence.
-  apply H0 in H1. break_exists; break_and.
-  eexists; split; eauto.
-Qed.
 
 Lemma find_funct_ptr_transf :
   forall b f,
     Genv.find_funct_ptr ge b = Some f ->
     exists f',
-      transf_fundef malloc_id f = OK f' /\
-      Genv.find_funct_ptr tge b = Some f'.
+      Genv.find_funct_ptr tge b = Some f' /\
+      transf_fundef malloc_id f = OK f'.
 Proof.
   intros.
-  app Genv.find_funct_ptr_transf_augment Genv.find_funct_ptr.
-  eauto.
+  eapply Genv.find_funct_ptr_transf_partial in H; eauto.
 Qed.
-
+(*
 Lemma find_funct_transf :
   forall vf vf',
     Val.lessdef vf vf' ->
@@ -402,7 +349,7 @@ Proof.
   break_match; try congruence.
   eapply find_funct_ptr_transf; eauto.
 Qed.
-  
+*)  
 Lemma funsig_transf :
   forall fd fd',
     transf_fundef malloc_id (Internal fd) = OK fd' ->
@@ -413,6 +360,7 @@ Proof.
   simpl. reflexivity.
 Qed.
 
+(*
 Lemma nothing_public_added :
   forall id x,
     Genv.find_symbol ge id = None ->
@@ -432,6 +380,7 @@ Proof.
 
   eauto.
 Qed.
+ *)
 
 Lemma public_symbol_transf :
   forall id,
@@ -440,22 +389,32 @@ Proof.
   intros.
   unfold tge. unfold ge.
   unfold Genv.public_symbol.
-  symmetry. break_match.
-  app find_symbol_transf Genv.find_symbol.
-  unfold tge in *. collapse_match.
+  erewrite find_symbol_transf.
   repeat rewrite Genv.globalenv_public.
-  unfold transf_prog in *.
-  unfold transform_partial_augment_program in *.
-  eapply bind_inversion in TRANSF.
-  destruct TRANSF. destruct H0.
-  inversion H1. simpl. reflexivity.
+  unfold transf_prog in *. 
+  erewrite transform_partial_program_public; eauto.
+Qed.  
 
-  break_match; eauto.
-  eapply nothing_public_added in Heqo; eauto.
-  destruct (in_dec ident_eq id (Genv.genv_public (Genv.globalenv tprog))); simpl; try congruence.
-  unfold tge in *. apply Heqo in i. inv_false.
+Lemma external_call_transf :
+  forall v m t vres m',
+    external_call EF_malloc ge (v :: nil) m t vres m' ->
+    external_call EF_malloc tge (v :: nil) m t vres m'.
+Proof.
+  intros.
+  inv H.
+  econstructor; eauto.
 Qed.
 
+
+Lemma malloc_dec_eq :
+  forall ef,
+    {ef = EF_malloc } + {ef <> EF_malloc}.
+Proof.
+  intros.
+  eapply (external_function_eq ef EF_malloc); eauto.
+Defined.
+
+(*
 Lemma external_call_transf :
   forall v m t vres m',
     external_call EF_malloc ge (v :: nil) m t vres m' ->
@@ -474,6 +433,7 @@ Proof.
   econstructor; eauto.
   split; eauto.
 Qed.
+ *)
 
 Lemma match_call_cont :
   forall k k',
@@ -483,50 +443,6 @@ Proof.
   induction 1; intros; simpl; try econstructor; eauto.
 Qed.
 
-Lemma env_lessdef_set_locals :
-  forall e e',
-    env_lessdef e e' ->
-    forall l,
-      env_lessdef (set_locals l e) (Cmajor.set_locals l e').
-Proof.
-  induction l; intros.
-  simpl. assumption.
-  simpl. eapply env_lessdef_set; eauto.
-Qed.
-
-Lemma norepet_tprog :
-  list_norepet (prog_defs_names tprog).
-Proof.
-  unfold transf_prog in *.
-  unfold transform_partial_augment_program in *.
-  eapply bind_inversion in TRANSF.
-  destruct TRANSF.
-  clear TRANSF.
-  break_and. inv H0.
-  clear H0.
-  unfold prog_defs_names.
-  simpl.
-
-Admitted.
-
-Lemma find_malloc_symbol :
-  exists b,
-    Genv.find_symbol tge malloc_id = Some b /\
-    Genv.find_funct_ptr tge b = Some (External (EF_malloc)).
-Proof.
-Admitted.
-
-Lemma env_lessdef_set_params :
-  forall ids vs vs',
-    Val.lessdef_list vs vs' ->
-    env_lessdef (set_params vs ids) (Cmajor.set_params vs' ids).
-Proof.
-  induction ids; intros.
-  simpl. unfold env_lessdef. intros. rewrite PTree.gempty in H0. congruence.
-  inversion H. remember tprog. subst. simpl. eapply env_lessdef_set; eauto.
-  simpl. eapply env_lessdef_set; eauto.
-Qed.
-
 Lemma single_step_correct:
   forall S1 t S2, Dflatmajor.step ge S1 t S2 ->
   forall T1, match_states S1 T1 ->
@@ -534,218 +450,91 @@ Lemma single_step_correct:
 Proof.
   induction 1; intros; invp match_states;
     try solve [simpl; inv MC; eexists; split; try eapply plus_one; try econstructor; eauto];
-    remember tprog; subst.
-  * (* return *)
-    eapply Mem.free_parallel_extends in ME; eauto.
-    break_exists. break_and.
-    eexists; split;
-      try eapply plus_one; econstructor; eauto.
-    eapply is_call_cont_transf; eauto.
-  * (* assign *)
-    eapply eval_expr_transf in H; eauto.
-    break_exists. break_and.
-    eexists; split; try eapply plus_one; try econstructor; eauto.
-    eapply env_lessdef_set; eauto.
-  * (* store *)
-    eapply eval_expr_transf in H; eauto.
-    eapply eval_expr_transf in H0; eauto.
-    repeat break_exists; repeat break_and.
-    eapply Mem.storev_extends in ME; eauto.
-    repeat break_exists; repeat break_and.
-    eexists; split; try eapply plus_one; try econstructor; eauto.
-  * (* call *)
-    eapply eval_expr_transf in H; eauto.
-    eapply eval_exprlist_transf in H0; eauto.
-    repeat break_exists. repeat break_and.
-    app find_funct_transf Genv.find_funct.
-    eexists; split; try eapply plus_one; try econstructor; eauto; simpl.
-    eapply funsig_transf; eauto.
-    econstructor; eauto.
-  * (* builtin *)
-    assert (t = E0) by (inv H0; eauto). subst t.
-    eapply eval_expr_transf in H; eauto.
-    break_exists; break_and.
-    eapply external_call_transf in H0; eauto.
-    break_exists; break_and.
-    name find_malloc_symbol Hmalloc.
-    break_exists; break_and.
-    eexists; split. eapply plus_left. econstructor; eauto.
-    econstructor; eauto. simpl.
-    collapse_match. reflexivity.
-    econstructor; eauto. econstructor; eauto.
-    simpl. find_rewrite. break_match; try congruence.
+    remember tprog; subst;
+      unfold Genv.find_funct in *;
+      repeat (break_match_hyp; try congruence); subst;
+        repeat match goal with
+               | [ H : eval_expr _ _ _ _ _ _ |- _ ] => eapply eval_expr_transf in H
+               | [ H : eval_exprlist _ _ _ _ _ _ |- _ ] => eapply eval_exprlist_transf in H
+               | [ H : external_call EF_malloc _ _ _ _ _ _ |- _ ] => eapply external_call_transf in H
+               end;
+                 try (eapply find_funct_ptr_transf in H1; repeat (break_exists; break_and));
+                 try solve [eapply plus_left_e;
+                            simpl;
+                            try solve [econstructor; eauto;
+                                       try eapply funsig_transf; eauto];
+                            try solve [eexists; split; try eapply star_refl;
+                                       solve [repeat (econstructor; eauto)]]];
+
+  try solve [eapply plus_left_e; simpl;
+             try solve [econstructor; eauto];
+             eexists; split; try eapply star_refl;
+             econstructor; eauto;
+             eapply match_call_cont; eauto].
+
+  (* turn malloc into external function call *)
+  * assert (t = E0) by (inv H0; congruence). subst t.
+    eapply plus_left_e. simpl.
+    repeat (econstructor; eauto).
+    erewrite find_symbol_transf; try collapse_match; eauto.
+    simpl. break_match; try congruence.
+    eapply find_funct_ptr_transf in malloc_block_malloc.
+    destruct malloc_block_malloc.
+    break_and. unfold transf_fundef in *. simpl in H3. inv H3.
+    eassumption.
     reflexivity.
-    reflexivity.
-    eapply star_left; nil_trace; try reflexivity.
-    econstructor; eauto.
-    eapply star_left; nil_trace; try reflexivity.
-    econstructor; eauto.
-    eapply star_refl.
-    reflexivity.
-    econstructor; eauto.
-    eapply env_lessdef_set; eauto.
-  * (* seq *)
-    simpl.
-    eexists; split; try eapply plus_one; try econstructor; eauto.
-    econstructor; eauto.
-  * (* block *)
-    simpl in *.
-    eexists; split; try eapply plus_one; try econstructor; eauto.
-    econstructor; eauto.
-  * (* switch *)
-    simpl.
-    eapply eval_expr_transf in H; eauto.
-    break_exists; break_and.
-    eexists; split; try eapply plus_one; try econstructor; eauto; simpl; eauto.
-    inv H0; inv H2; econstructor; eauto.
-  * (* return *)
-    simpl.
-    eapply Mem.free_parallel_extends in H; eauto.
-    break_exists; break_and.
-    eexists; split; try eapply plus_one; try econstructor;
-    eauto;
-    try eapply match_call_cont; eauto.
-    
-  * (* return *)
-    eapply eval_expr_transf in H; eauto.
-    eapply Mem.free_parallel_extends in H0; eauto.
-    repeat (break_exists; break_and).
-    eexists; split; try eapply plus_one; try econstructor; eauto; simpl; eauto.
-    eapply match_call_cont; eauto.
-    
-  * (* call internal *)
-    unfold transf_fundef in TF. inv TF.
-    eapply Mem.alloc_extends in H; eauto.
-    break_exists. break_and.
-    eexists; split; try eapply plus_one; nil_trace; try reflexivity;
-    econstructor; eauto.
-    eapply env_lessdef_set_locals.
-    eapply env_lessdef_set_params; eauto.
-    omega.
-    simpl. omega.
-  * (* return *)
-    inversion MC. remember tprog. subst.
-    eexists; split; try eapply plus_one; try econstructor; eauto; simpl; eauto.
-    destruct optid. simpl.
-    eapply env_lessdef_set; eauto.
-    simpl. assumption.
-Admitted.
 
+    eapply star_left_e.
+    econstructor; eauto.
+    eapply star_left_e.
+    econstructor; eauto.
+    eexists; split. eapply star_refl.
+    econstructor; eauto.
 
-Lemma alloc_drop_perm :
-  forall m lo hi m' b,
-    Mem.alloc m lo hi = (m',b) ->
-    exists m'',
-      Mem.drop_perm m' b lo hi Nonempty = Some m''.
-Proof.
-  intros.
-  unfold Mem.drop_perm.
-  break_match; try solve [eauto].
-  exfalso. apply n. unfold Mem.range_perm. intros.
-  app Mem.perm_alloc_2 Mem.alloc.
-Qed.  
-
-Lemma alloc_global_succeeds :
-  forall {F V : Type} (ge : Genv.t F V) i g m,
-  exists m',
-    Genv.alloc_global ge m (i,g) = Some m'.
-Proof.
-  intros. destruct g.
-  simpl;
-    break_let.
-  eapply alloc_drop_perm; eauto.
-  simpl.
-  break_let.
-  (* This is true but a pain in the ass *)
-Admitted.
-
-Lemma alloc_globals_succeeds :
-  forall {F V : Type} (ge : Genv.t F V) l m,
-    exists m',
-      Genv.alloc_globals ge m l = Some m'.
-Proof.
-  induction l; intros.
-  simpl. eauto.
-  simpl. destruct a.
-  edestruct (@alloc_global_succeeds F V).
-  rewrite H.
-  eapply IHl.
+  (* function call *)
+  * unfold transf_fundef in *.
+    find_inversion.
+    eapply plus_left_e.
+    econstructor; eauto.
+    eexists; split. eapply star_refl.
+    econstructor; eauto.
 Qed.
 
-Lemma init_mem_transf :
-  forall m,
-    Genv.init_mem prog = Some m ->
-    exists m',
-      Genv.init_mem tprog = Some m' /\ Mem.extends m m'.
+Lemma is_callstate_match :
+  forall fv av st',
+    Cmajor.is_callstate tprog fv av st' ->
+    exists st,
+      match_states st st' /\ is_callstate prog fv av st.
 Proof.
-  intros.
-  unfold transf_prog in TRANSF.
-  eapply Genv.init_mem_transf_augment in H; eauto.
-  rewrite H.
-  edestruct (@alloc_globals_succeeds Cmajor.fundef unit).
-  rewrite H0. eexists. split. reflexivity.
-  clear H.
-
-  admit. (* adding more globals extends the mem *)
-Admitted.
-(*
-Lemma match_final_state :
- forall (s1 : Smallstep.state (Dflatmajor.semantics prog))
-        (s2 : Smallstep.state (Cmajor.semantics tprog)) (r : int),
-   match_states s1 s2 ->
-   Smallstep.final_state (Dflatmajor.semantics prog) s1 r ->
-   Smallstep.final_state (Cmajor.semantics tprog) s2 r.
-Proof.
-  intros.
-  inv H0. inv H.
-  inv LD.
-  inv MC.
-  econstructor; eauto.
-Qed.
-
-Lemma initial_states_match :
-  forall s1 : Smallstep.state (Dflatmajor.semantics prog),
-    Smallstep.initial_state (Dflatmajor.semantics prog) s1 ->
-    exists s2 : Smallstep.state (Cmajor.semantics tprog),
-      Smallstep.initial_state (Cmajor.semantics tprog) s2 /\ match_states s1 s2.
-Proof.
-  intros. 
-  inversion H.
-  eapply init_mem_transf in H0; try reflexivity.
-  break_exists; break_and.
+  intros. inv H.
+  eapply Genv.find_funct_ptr_rev_transf_partial in H2; eauto.
+  break_exists. break_and.
   eexists; split; econstructor; eauto;
-    simpl; try solve [econstructor; eauto].
-  erewrite find_symbol_transf; eauto.
-  unfold transf_prog in TRANSF.
-  erewrite transform_partial_augment_program_main; eauto.
-  app find_funct_ptr_transf Genv.find_funct_ptr.
-  unfold tge in *. find_rewrite.
-  unfold transf_fundef in *. congruence.
-  eauto.
-Qed.  
-*)
+    try solve [repeat (econstructor; eauto)].
+  
+  
+Admitted.
+
+Lemma match_final_states :
+  forall st st' r,
+    match_states st st' ->
+    final_state prog st r ->
+    Cmajor.final_state tprog st' r.
+Proof.
+Admitted.
+
 Theorem fsim :
   forward_simulation (Dflatmajor.semantics prog) (Cmajor.semantics tprog).
 Proof.
-Admitted.
-
+  eapply forward_simulation_plus.
+  intros. eapply is_callstate_match; eauto.
+  instantiate (1 := eq) in H0. subst. eauto.
+  intros. exists v1; split; eauto. eapply match_final_states; eauto.
+  eapply single_step_correct; eauto.
+Qed.
 
 End PRESERVATION.
 
 
-Theorem transf_program_correct:
-  forall prog tprog,
-    list_norepet (prog_defs_names prog) ->
-    (forall id : ident, In id (map fst (new_globs (Pos.succ (malloc_id prog)) (malloc_id prog))) ->
-                        ~ In id (Genv.genv_public (Genv.globalenv tprog))) ->
-    transf_prog prog = OK tprog ->
-    forward_simulation (Dflatmajor.semantics prog) (Cmajor.semantics tprog).
-Proof.
-  intros.
-  eapply forward_simulation_plus.
-  admit.
-  admit.
-  eapply single_step_correct; eauto.
-Admitted.
 
 
